WIP: bind of 2-index RST

ulib/LowStar.RST.TwoIndex.fst
@@ -31,33 +31,40 @@ assume val lemma_loc_not_unused_in_modifies_includes (l0 l1:B.loc) (h0 h1:HS.mem
                      B.loc_includes l1 l0 /\ B.modifies l1 h0 h1))
           (ensures  (B.loc_includes (B.loc_not_unused_in h1) l1))
 
+(* Another (currently assumed) lemma *)
+assume val lemma_modifies_loc_disjoint (l0 l1:B.loc) (h0 h1 h2:HS.mem) 
+  : Lemma (requires (B.modifies l0 h0 h1 /\
+                     B.modifies l1 h1 h2 /\ 
+                     (forall l . B.loc_disjoint l l0 ==> B.loc_disjoint l l1)))
+          (ensures  (B.modifies l0 h0 h2))
+
 (* Abstract modifies clause for the resource-indexed state effect *)
 
 abstract
-let modifies (res:resource) (h0 h1:HS.mem) =
-    B.modifies (as_loc (fp res)) h0 h1 /\
-    HST.equal_domains h0 h1
+let modifies (res0 res1:resource) (h0 h1:HS.mem) =
+    B.modifies (as_loc (fp res0)) h0 h1 /\ 
+    (forall l . B.loc_disjoint l (as_loc (fp res0)) ==> B.loc_disjoint l (as_loc (fp res1)))
 
 let modifies_refl (res:resource) (h:HS.mem) 
-  : Lemma (modifies res h h)
-           [SMTPat (modifies res h h)]
+  : Lemma (modifies res res h h)
+           [SMTPat (modifies res res h h)]
   = ()
 
-let modifies_trans (res0 res1:resource) (h0 h1 h2:HS.mem) 
+let modifies_trans (res0 res1 res2:resource) (h0 h1 h2:HS.mem) 
   : Lemma (requires 
-             modifies res0 h0 h1 /\
-             modifies res1 h1 h2)
+             modifies res0 res1 h0 h1 /\
+             modifies res1 res2 h1 h2)
            (ensures
-             modifies (r_union res0 res1) h0 h2)
-           [SMTPat (modifies (r_union res0 res1) h0 h2);
-            SMTPat (modifies res0 h0 h1)]
-  = ()
+             modifies res0 res2 h0 h2)
+           [SMTPat (modifies res0 res2 h0 h2);
+            SMTPat (modifies res0 res1 h0 h1)] =
+  lemma_modifies_loc_disjoint (as_loc (fp res0)) (as_loc (fp res1)) h0 h1 h2
 
 let reveal_modifies ()
-  : Lemma (forall res h0 h1.{:pattern modifies res h0 h1}
-             modifies res h0 h1 <==>
-             B.modifies (as_loc (fp res)) h0 h1 /\
-             HST.equal_domains h0 h1)
+  : Lemma (forall res0 res1 h0 h1.{:pattern modifies res0 res1 h0 h1}
+             modifies res0 res1 h0 h1 <==>
+             B.modifies (as_loc (fp res0)) h0 h1 /\
+             (forall frame . B.loc_disjoint frame (as_loc (fp res0)) ==> B.loc_disjoint frame (as_loc (fp res1))))
   = ()
 
 (* State effect indexed by resources *)
@@ -76,12 +83,12 @@ let reveal_rst_inv ()
              B.loc_includes (B.loc_not_unused_in h) (as_loc (fp res)))
   = ()
 
-let ret_resource res0 a =
+let post_resource res0 a =
   a -> res1:resource{(forall frame . r_disjoint frame res0 ==> r_disjoint frame res1)}
 
 effect RST (a:Type)
            (res0:resource)                                      //Pre-resource (expected from the caller)
-           (res1:ret_resource res0 a)                           //Post-resource (returned back to the caller)
+           (res1:post_resource res0 a)                          //Post-resource (returned back to the caller)
            (pre:r_pre res0)
            (post:r_post res0 a res1) = 
        STATE a
@@ -93,9 +100,38 @@ effect RST (a:Type)
                (forall (x:a) (h1:HS.mem).
                  inv (res1 x) h1 /\                              //Ensure the post-resource invariant
                  rst_inv (res1 x) h1 /\                          //Ensure the additional footprints invariant
-                 modifies (r_union res0 (res1 x)) h0 h1 /\       //Ensure that at most resources' footprints are modified
+                 modifies res0 (res1 x) h0 h1 /\       //Ensure that at most resources' footprints are modified
                  post h0 x h1 ==>                                //Ensure the post-condition
                  k x h1))                                        //Prove the continuation under this hypothesis
+
+(* Bind operation for RST *)
+
+(*
+let lemma_ret_resource (#a #b:Type)
+                       (res0:resource)
+                       (res1:(a -> res1:resource{(forall frame . r_disjoint frame res0 ==> r_disjoint frame res1)}))
+                       (res2:resource{forall frame x . r_disjoint frame (res1 x) ==> r_disjoint frame res2})
+                       (frame:resource)
+ : Lemma (requires (r_disjoint frame res0))
+         (ensures  (r_disjoint frame res2)) = 
+  assert (forall x . r_disjoint frame (res1 x));
+  assert (forall x . r_disjoint frame (res1 x) ==> r_disjoint frame res2);
+  admit ()
+*)
+
+let bind (#a #b:Type)
+         (#res0:resource)
+         (#res1:post_resource res0 a)
+         (#res2:(b -> res2:resource{(forall frame x . r_disjoint frame (res1 x) ==> r_disjoint frame res2) /\
+                                    (forall frame . r_disjoint frame res0 ==> r_disjoint frame res2)}))       // TODO: this ought to be provable from other assumptions
+         (#pre0:r_pre res0)
+         (#post0:r_post res0 a res1)
+         (#post1:(x:a -> r_post (res1 x) b res2))
+         (f:unit -> RST a res0 res1 pre0 post0)
+         (g:(x:a -> RST b (res1 x) res2 (fun h1 -> exists h0 . post0 h0 x h1) (post1 x)))
+       : RST b res0 res2 pre0 (fun h0 y h2 -> exists x h1 . post0 h0 x h1 /\ post1 x h1 y h2) = 
+  g (f ())
+
 
 (* Generic framing operation for RST (through resource inclusion) *)
 
@@ -107,35 +143,36 @@ let frame_pre (#outer0:resource)
               (h:imem (inv outer0)) =
   pre h
 
+// The pre- and post deltas are the same
 let frame_post_delta (#outer0:resource)
                      (#inner0:resource)
                      (delta0:r_includes outer0 inner0)
                      (a:Type)
-                     (outer1:ret_resource outer0 a)
-                     (inner1:ret_resource inner0 a) =
+                     (outer1:post_resource outer0 a)
+                     (inner1:post_resource inner0 a) =
   x:a -> delta1:r_includes (outer1 x) (inner1 x){delta0 == delta1}
 
 unfold
 let frame_post (#outer0:resource)
                (#inner0:resource)
                (#a:Type)
-               (#outer1:ret_resource outer0 a)
-               (#inner1:ret_resource inner0 a)
+               (#outer1:post_resource outer0 a)
+               (#inner1:post_resource inner0 a)
                (delta0:r_includes outer0 inner0)
                (delta1:frame_post_delta delta0 a outer1 inner1)
                (post:r_post inner0 a inner1)
                (h0:imem (inv outer0))
                (x:a)
                (h1:imem (inv (outer1 x))) = 
-  delta0 == delta1 x /\ // to trigger the refinement on (delta1 x)
+  delta0 == delta1 x /\ // here to trigger the refinement on (delta1 x)
   post h0 x h1 /\
   sel (view_of delta0) h0 == sel (view_of (delta1 x)) h1
 
 let frame (#outer0:resource)
           (#inner0:resource)
           (#a:Type)
-          (#outer1:ret_resource outer0 a)
-          (#inner1:ret_resource inner0 a)
+          (#outer1:post_resource outer0 a)
+          (#inner1:post_resource inner0 a)
           (delta0:r_includes outer0 inner0)
           (delta1:frame_post_delta delta0 a outer1 inner1)
           (#pre:r_pre inner0)
@@ -147,7 +184,7 @@ let frame (#outer0:resource)
   let h0 = get () in 
   let x = f () in 
   let h1 = get () in 
-  assert (delta0 == delta1 x); // to trigger the refinement on (delta1 x)
+  assert (delta0 == delta1 x); // here to trigger the refinement on (delta1 x)
   lemma_loc_not_unused_in_modifies_includes 
     (as_loc (fp outer0)) 
     (as_loc (fp (r_union outer0 (outer1 x)))) 
